theories/instructions/stp_test.v
@@ -6,23 +6,23 @@ Require Import isla.instructions.stp.
 Definition start_address := [BV{64} (0x0000000010300000 - 0x4)].
 Definition spec : list seq_label := [ SInstrTrap [BV{64} 0x0000000010300004] ].
 
-Definition sys_regs `{!islaG Σ} `{!threadG} : iProp Σ :=
-  ("SCTLR_EL2" ↦ᵣ Val_Bits [BV{64} 0x0000000004000002] ∗
-  "SCR_EL3" ↦ᵣ Val_Bits [BV{32} 0] ∗
-  "TCR_EL2" ↦ᵣ Val_Bits [BV{64} 0] ∗
-  "CFG_ID_AA64PFR0_EL1_EL0" ↦ᵣ Val_Bits [BV{4} 1] ∗
-  "CFG_ID_AA64PFR0_EL1_EL1" ↦ᵣ Val_Bits [BV{4} 1] ∗
-  "CFG_ID_AA64PFR0_EL1_EL2" ↦ᵣ Val_Bits [BV{4} 1] ∗
-  "CFG_ID_AA64PFR0_EL1_EL3" ↦ᵣ Val_Bits [BV{4} 1] ∗
-  "OSLSR_EL1" ↦ᵣ Val_Bits [BV{32} 0] ∗
-  "OSDLR_EL1" ↦ᵣ Val_Bits [BV{32} 0] ∗
-  "EDSCR" ↦ᵣ Val_Bits [BV{32} 0] ∗
-  "MPIDR_EL1" ↦ᵣ Val_Bits [BV{64} 0] ∗
-  "PSTATE" @ "SP" ↦ᵣ Val_Bits [BV{1} 1] ∗
-  "PSTATE" @ "EL" ↦ᵣ Val_Bits [BV{2} 2] ∗
-  "PSTATE" @ "nRW" ↦ᵣ Val_Bits [BV{1} 0] ∗
-  "PSTATE" @ "D" ↦ᵣ Val_Bits [BV{1} 1]
-)%I.
+Definition sys_regs : list (reg_col_entry * valu) := [
+  (RegColDirect "SCTLR_EL2" , Val_Bits [BV{64} 0x0000000004000002] );
+  (RegColDirect "SCR_EL3" , Val_Bits [BV{32} 0] );
+  (RegColDirect "TCR_EL2" , Val_Bits [BV{64} 0] );
+  (RegColDirect "CFG_ID_AA64PFR0_EL1_EL0" , Val_Bits [BV{4} 1] );
+  (RegColDirect "CFG_ID_AA64PFR0_EL1_EL1" , Val_Bits [BV{4} 1] );
+  (RegColDirect "CFG_ID_AA64PFR0_EL1_EL2" , Val_Bits [BV{4} 1] );
+  (RegColDirect "CFG_ID_AA64PFR0_EL1_EL3" , Val_Bits [BV{4} 1] );
+  (RegColDirect "OSLSR_EL1" , Val_Bits [BV{32} 0] );
+  (RegColDirect "OSDLR_EL1" , Val_Bits [BV{32} 0] );
+  (RegColDirect "EDSCR" , Val_Bits [BV{32} 0] );
+  (RegColDirect "MPIDR_EL1" , Val_Bits [BV{64} 0] );
+  (RegColStruct "PSTATE" "SP" , Val_Bits [BV{1} 1] );
+  (RegColStruct "PSTATE" "EL" , Val_Bits [BV{2} 2] );
+  (RegColStruct "PSTATE" "nRW" , Val_Bits [BV{1} 0] );
+  (RegColStruct "PSTATE" "D" , Val_Bits [BV{1} 1])
+].
 
 Definition cont_spec `{!islaG Σ} `{!threadG} a sp (v1 v2 : bv 64) : iProp Σ :=
   ∃ (vold1 vold2 : bv 64),
@@ -32,12 +32,12 @@ Definition cont_spec `{!islaG Σ} `{!threadG} a sp (v1 v2 : bv 64) : iProp Σ :=
   (bv_sub sp [BV{64} 8]) ↦ₘ vold2 ∗
   ⌜bv_unsigned sp < 2 ^ 52⌝ ∗
   "SP_EL2" ↦ᵣ Val_Bits sp ∗
-  sys_regs ∗
+  reg_col sys_regs ∗
   instr_pre a (
     "R0" ↦ᵣ Val_Bits v1 ∗
     "R1" ↦ᵣ Val_Bits v2 ∗
     "SP_EL2" ↦ᵣ Val_Bits (bv_sub sp [BV{64} 16])∗
-    sys_regs ∗
+    reg_col sys_regs ∗
     (bv_sub sp [BV{64} 16]) ↦ₘ v1 ∗
     (bv_sub sp [BV{64} 8]) ↦ₘ v2 ∗
     True).
@@ -47,8 +47,8 @@ Lemma stp_wp `{!islaG Σ} `{!threadG} (sp v1 v2: bv 64):
   instr_body 0x0000000010300000 (cont_spec 0x0000000010300004 sp v1 v2).
 Proof.
   iStartProof.
-  unfold cont_spec, sys_regs.
+  unfold cont_spec.
   repeat liAStep; liShow.
   Unshelve.
-  all: try (repeat f_equal; unLET; bv_solve).
+  all: try (repeat f_equal; bv_solve).
 Qed.
